More serializer work

src/parse/Input.v
@@ -4,6 +4,7 @@ From Pollux.parse Require Import Util.
 (* Define abstract types and their properties *)
 Module Type AbstractInput.
   Parameter Input : Type.
+  Parameter Input_default : Input.
   Parameter C : Type.
   Parameter C_default : C.
 
@@ -27,6 +28,14 @@ Module Type AbstractInput.
   Axiom CharAt_correct :
     forall self i, 0 <= i < Length self ->
     CharAt self i = nth i (View self) C_default.
+
+  Parameter App : Input -> Input -> Input.
+  Axiom App_correct :
+    forall self other, App self other = ToInput $ (View self) ++ (View other).
+  Axiom App_nil_l :
+    forall self, App Input_default self = self.
+  Axiom App_assoc :
+    forall i1 i2 i3, App (App i1 i2) i3 = App i1 (App i2 i3).
 
   (* AbstractInput must support dropping elements *)
   Parameter Drop : Input -> nat -> Input.
@@ -52,6 +61,7 @@ Module ByteInput <: AbstractInput.
   Definition C := byte.
   Definition C_default := (W8 0).
   Definition Input := list C.
+  Definition Input_default : Input := [].
 
   Definition C_eq := w8_eq_dec.
   Definition Input_eq := @list_eq_dec C C_eq.
@@ -60,27 +70,37 @@ Module ByteInput <: AbstractInput.
   Definition View (self : Input) := self.
   Definition Length (self : Input) := length self.
   Definition CharAt (self : Input) (i : nat) := nth i self C_default.
+  Definition App (self : Input) (other : Input) := self ++ other.
   Definition Drop (self : Input) (start : nat) := drop start self.
   Definition Slice (self : Input) (start last : nat) := Util.sublist start last self.
 
   Theorem View_length : forall self, length (View self) = Length self.
-  Proof. intros. reflexivity. Qed.
+  Proof. reflexivity. Qed.
 
   Theorem ToInput_correct : forall r, View (ToInput r) = r.
-  Proof. intros. reflexivity. Qed.
+  Proof. reflexivity. Qed.
 
   Theorem CharAt_correct : forall self i, 0 <= i < length self ->
                                      CharAt self i = nth i (View self) C_default.
-  Proof. intros. reflexivity. Qed.
+  Proof. reflexivity. Qed.
+
+  Theorem App_correct : forall self other, App self other = ToInput $ (View self) ++ (View other).
+  Proof. reflexivity. Qed.
+
+  Theorem App_nil_l : forall self, App Input_default self = self.
+  Proof. intros. unfold App. rewrite app_nil_l. reflexivity. Qed.
+
+  Theorem App_assoc : forall i1 i2 i3, App (App i1 i2) i3 = App i1 (App i2 i3).
+  Proof. intros. unfold App. rewrite <- app_assoc. reflexivity. Qed.
 
   Theorem Drop_correct : forall self start, 0 <= start <= Length self ->
                                        View (Drop self start) = drop start (View self).
-  Proof. intros. reflexivity. Qed.
+  Proof. reflexivity. Qed.
 
   Theorem Slice_correct : forall self start end',
     0 <= start /\ start <= end' /\ end' <= Length self ->
     View (Slice self start end') = Util.sublist start end' (View self).
-  Proof. intros. reflexivity. Qed.
+  Proof. reflexivity. Qed.
 
   Theorem Drop_zero : forall self, Drop self 0 = self.
   Proof. intros. unfold Drop. apply drop_0. Qed.
@@ -96,4 +116,3 @@ Module ByteInput <: AbstractInput.
   Qed.
 
 End ByteInput.
-
